Veir/PatternRewriter/Lemmas.lean
@@ -1,0 +1,18 @@
+module
+
+public import Veir.PatternRewriter.Basic
+
+public section
+namespace Veir
+
+variable {OpInfo : Type} [HasOpInfo OpInfo]
+
+namespace PatternRewriter
+
+@[simp, grind =]
+theorem replaceValue_ctx {rewriter : PatternRewriter OpInfo} {oldVal newVal : ValuePtr}
+    {neValues : oldVal ≠ newVal} {oldIn : oldVal.InBounds rewriter.ctx.raw}
+    {newIn : newVal.InBounds rewriter.ctx.raw} :
+    (rewriter.replaceValue oldVal newVal neValues oldIn newIn).ctx
+      = WfRewriter.replaceValue rewriter.ctx oldVal newVal neValues oldIn newIn := by
+  simp [replaceValue, addUsersInWorklist_same_ctx]
